### 基本积分公式
##### 幂函数和指数函数
- $\displaystyle\int x^k\mathrm dx=\frac{1}{k+1}x^{k+1}+C,k\neq -1;\;\begin{cases}\int\frac{1}{x^2}\mathrm dx=-\frac{1}{x}+C\\[2ex]\int\frac{1}{\sqrt{x}}\mathrm dx=2\sqrt{x}+C\end{cases}$
- $\displaystyle\int\frac{1}{x}\mathrm dx=\ln |x|+C$
- $\displaystyle\int\mathrm e^x\mathrm dx=\mathrm e^x+C$
- $\displaystyle\int a^x\mathrm dx=\frac{a^x}{\ln a}+C,\; a>0\text{且}a\neq 1$
##### 三角函数
- $\displaystyle\int\sin x\mathrm dx=-\cos x+C$
- $\displaystyle\int\cos x\mathrm dx=\sin x+C$
- $\displaystyle\int\tan x\mathrm dx=-\ln\left|\cos x\right|+C$
- $\displaystyle\int\cot x\mathrm dx=\ln\left|\sin x\right|+C$
- $\displaystyle\int\sec x\mathrm dx=\int\frac{\mathrm dx}{\cos x}=\ln\left|\sec x+\tan x\right|+C$
- $\displaystyle\int\csc x\mathrm dx=\int\frac{\mathrm dx}{\sin x}=\ln\left|\csc x-\cot x\right|+C$
- $\displaystyle\int\sin^2 x\mathrm dx=\int\frac{1-\cos 2x}{x}\mathrm dx=\frac x2-\frac{\sin 2x}4+C$
- $\displaystyle\int\cos^2 x\mathrm dx=\int\frac{1+\cos 2x}{x}\mathrm dx=\frac x2+\frac{\sin 2x}4+C$
- $\displaystyle\int\tan^2 x\mathrm dx=\int(\sec^2x-1)\mathrm dx=\tan x-x+C$
- $\displaystyle\int\cot^2 x\mathrm dx=\int(\csc^2x-1)\mathrm dx=-\cot x-x+C$
- $\displaystyle\int\sec^2 x\mathrm dx=\tan x+C$
- $\displaystyle\int\csc^2 x\mathrm dx=-\cot x+C$
##### 分式
- $\displaystyle\int\frac 1{1+x^2}\mathrm dx=\arctan x+C$
- $\displaystyle\int\frac 1{a^2+x^2}\mathrm dx=\frac 1a\arctan\frac xa+C(a>0)$
- $\displaystyle\int\frac 1{\sqrt{1-x^2}}\mathrm dx=\arcsin x+C$
- $\displaystyle\int\frac 1{\sqrt{a^2-x^2}}\mathrm dx=\arcsin\frac xa+C(a>0)$
- $\displaystyle\int\frac 1{\sqrt{x^2+a^2}}\mathrm dx=\ln\left(x+\sqrt{x^2+a^2}\right)+C$（常见$a=1$）
- $\displaystyle\int\frac 1{\sqrt{x^2-a^2}}\mathrm dx=\ln\left|x+\sqrt{x^2-a^2}\right|+C$（$|x|>|a|$）
- $\displaystyle\int\frac 1{x^2-a^2}\mathrm dx=\frac 1{2a}\ln\left|\frac{x-a}{x+a}\right|+C$
- $\displaystyle\int\frac 1{a^2-x^2}\mathrm dx=\frac 1{2a}\ln\left|\frac{x+a}{x-a}\right|+C$
- $\displaystyle\int\sqrt{a^2-x^2}\mathrm dx=\frac{a^2}2\arcsin\frac xa+\frac x2\sqrt{a^2-x^2}+C$（$a>|x|\ge 0$）
### 常用的凑微分公式
- $\displaystyle x\mathrm dx=\frac 12\mathrm d(x^2)\Longrightarrow\int xf(x^2)\mathrm dx=\frac 12\int f(x^2)\mathrm d(x^2)\xlongequal{u=x^2}\frac 12\int f(u)\mathrm du$
- $\displaystyle\sqrt{x}\mathrm dx=\frac23 \mathrm d(x^{\frac32})\Longrightarrow\int\sqrt{x}f\left(x^{\frac 32}\right)\mathrm dx=\frac 23\int f\left(x^{\frac 32}\right)\mathrm d(x^{\frac32})\xlongequal{u=x^{\frac32}}\frac 23\int f(u)\mathrm du$
- $\displaystyle\frac 1{\sqrt x}\mathrm dx=2\mathrm d(\sqrt x)\Longrightarrow\int \frac 1{\sqrt x}f(\sqrt x)\mathrm dx=2\int f(\sqrt x)\mathrm d(\sqrt x)\xlongequal{u=\sqrt x}2\int f(u)\mathrm du$
- $\displaystyle\frac 1{x^2}\mathrm dx=\mathrm d\left(-\frac 1x\right)\Longrightarrow\int\frac 1{x^2}f\left(-\frac 1x\right)\mathrm dx=\int f\left(-\frac 1x\right)\mathrm d\left(-\frac 1x\right)\xlongequal{u=-\frac 1x}\int f(u)\mathrm du$
- $\displaystyle\frac 1x\mathrm dx=\mathrm d(\ln x)\Longrightarrow\int\frac 1xf(\ln x)\mathrm dx=\int f(\ln x)\mathrm d(\ln x)\xlongequal{u= \ln x}\int f(u)\mathrm du$
- $\displaystyle\mathrm e^x\mathrm dx=\mathrm d(\mathrm e^x)\Longrightarrow\int \mathrm e^xf(\mathrm e^x)\mathrm dx=\int f(\mathrm e^x)\mathrm d(\mathrm e^x)\xlongequal{u=\mathrm e^x}\int f(u)\mathrm du$
- $\displaystyle a^x\mathrm dx=\frac 1{\ln a}\mathrm d(a^x)\Longrightarrow\int a^xf(a^x)\mathrm dx=\frac 1{\ln a}\int f(a^x)\mathrm d(a^x)\xlongequal{u=a^x}\frac 1{\ln a}\int f(u)\mathrm du$
- $\displaystyle\sin x\mathrm dx=\mathrm d(-\cos x)\Longrightarrow\int\sin x\cdot f(-\cos x)\mathrm dx=\int f(-\cos x)\mathrm d(-\cos x)\xlongequal{u=-\cos x}\int f(u)\mathrm du$
- $\displaystyle\cos x\mathrm dx=\mathrm d(\sin x)\Longrightarrow\int\cos x\cdot f(\sin x)\mathrm dx=\int f(\sin x)\mathrm d(\sin x)\xlongequal{u=\sin x}\int f(u)\mathrm du$
- $\displaystyle\frac 1{\cos^2x}\mathrm dx=\mathrm d(\tan x)\Longrightarrow\int\frac{f(\tan x)}{\cos^2x}\mathrm dx=\int f(\tan x)\mathrm d(\tan x)\xlongequal{u=\tan x}\int f(u)\mathrm du$
- $\displaystyle\frac 1{\sin^2x}\mathrm dx=\mathrm d(-\cot x)\Longrightarrow\int\frac{f(-\cot x)}{\sin^2x}\mathrm dx=\int f(-\cot x)\mathrm d(-\cot x)\xlongequal{u=-\cot x}\int f(u)\mathrm du$
- $\displaystyle\frac 1{1+x^2}\mathrm dx=\mathrm d(\arctan x)\Longrightarrow\int\frac{f(\arctan x)}{1+x^2}\mathrm dx=\int f(\arctan x)\mathrm d(\arctan x)\xlongequal{u=\arctan x}\int f(u)\mathrm du$
- $\displaystyle\frac 1{\sqrt{1+x^2}}\mathrm dx=\mathrm d(\arcsin x)\Longrightarrow\int\frac{f(\arcsin x)}{\sqrt{1+x^2}}\mathrm dx=\int f(\arcsin x)\mathrm d(\arcsin x)\xlongequal{u=\arcsin x}\int f(u)\mathrm du$
